refine: ArchAcc_R given Arch prefix
In preparation for arch-split.
Create ArchAcc_R.thy and update import hierarchy.

Signed-off-by: Rafal Kolanski <rafal.kolanski@proofcraft.systems>

proof/refine/RISCV64/ArchArchAcc_R.thy
@@ -1,16 +1,13 @@
 (*
- * Copyright 2023, Proofcraft Pty Ltd
  * Copyright 2020, Data61, CSIRO (ABN 41 687 119 230)
  *
  * SPDX-License-Identifier: GPL-2.0-only
  *)
 
-(*
-  Lemmas on arch get/set object etc
-*)
+(* Arch-specific lemmas on arch get/set object etc *)
 
-theory ArchAcc_R
-imports SubMonad_R
+theory ArchArchAcc_R
+imports ArchAcc_R
 begin
 
 unbundle l4v_word_context
@@ -20,11 +17,11 @@ context begin interpretation Arch . (*FIXME: arch-split*)
 declare if_cong[cong] (* FIXME: if_cong *)
 
 lemma asid_pool_at_ko:
-  "asid_pool_at p s \<Longrightarrow> \<exists>pool. ko_at (ArchObj (AARCH64_A.ASIDPool pool)) p s"
+  "asid_pool_at p s \<Longrightarrow> \<exists>pool. ko_at (ArchObj (RISCV64_A.ASIDPool pool)) p s"
   by (clarsimp simp: asid_pools_at_eq obj_at_def elim!: opt_mapE)
 
-lemma corres_gets_asid:
-  "corres (\<lambda>a c. a = c o ucast) \<top> \<top> (gets asid_table) (gets (armKSASIDTable \<circ> ksArchState))"
+lemma corres_gets_asid[corres]:
+  "corres (\<lambda>a c. a = c o ucast) \<top> \<top> (gets (riscv_asid_table \<circ> arch_state)) (gets (riscvKSASIDTable \<circ> ksArchState))"
   by (simp add: state_relation_def arch_state_relation_def)
 
 lemma asid_low_bits [simp]:
@@ -55,6 +52,7 @@ lemma pspace_aligned_cross:
   apply clarsimp
   apply (rename_tac ko' a a' P ko)
   apply (erule (1) obj_relation_cutsE; clarsimp simp: objBits_simps)
+
        \<comment>\<open>CNode\<close>
        apply (clarsimp simp: cte_map_def)
        apply (simp only: cteSizeBits_def cte_level_bits_def)
@@ -62,18 +60,23 @@ lemma pspace_aligned_cross:
         apply (erule is_aligned_weaken, simp)
        apply (rule is_aligned_weaken)
         apply (rule is_aligned_shiftl_self, simp)
+
       \<comment>\<open>TCB\<close>
       apply (clarsimp simp: tcbBlockSizeBits_def elim!: is_aligned_weaken)
+
      \<comment>\<open>PageTable\<close>
+     apply (clarsimp simp: archObjSize_def pteBits_def table_size_def ptTranslationBits_def pte_bits_def)
      apply (rule is_aligned_add)
       apply (erule is_aligned_weaken)
-      apply (simp add: bit_simps)
+      apply simp
      apply (rule is_aligned_shift)
+
     \<comment>\<open>DataPage\<close>
     apply (rule is_aligned_add)
      apply (erule is_aligned_weaken)
      apply (rule pbfs_atleast_pageBits)
-    apply (rule is_aligned_shift)
+   apply (rule is_aligned_shift)
+
    \<comment>\<open>Other non-arch\<close>
    apply (simp add: other_obj_relation_def)
    apply (clarsimp simp: bit_simps' tcbBlockSizeBits_def epSizeBits_def ntfnSizeBits_def
@@ -100,10 +103,8 @@ lemma obj_relation_cuts_range_limit:
       apply (rule_tac x=tcbBlockSizeBits in exI)
       apply (simp add: tcbBlockSizeBits_def)
      apply (rule_tac x=pte_bits in exI)
-     apply (simp add: is_aligned_shift mask_def)
-     apply (rule shiftl_less_t2n)
-      apply (simp add: table_size_def)
-     apply (simp add: bit_simps)
+     apply (simp add: bit_simps is_aligned_shift mask_def)
+     apply word_bitwise
     apply (rule_tac x=pageBits in exI)
     apply (simp add: is_aligned_shift pbfs_atleast_pageBits)
     apply (simp add: mask_def shiftl_t2n mult_ac)
@@ -195,8 +196,8 @@ lemma asid_pool_at_cross:
    apply clarsimp
   apply (clarsimp simp: pspace_relation_def)
   apply (drule bspec, fastforce)
-  apply (clarsimp simp: other_aobj_relation_def objBits_simps
-                  split: kernel_object.splits arch_kernel_object.splits)
+  apply (clarsimp simp: other_aobj_relation_def split: kernel_object.splits arch_kernel_object.splits)
+  apply (clarsimp simp: objBits_simps)
   apply (frule (1) pspace_alignedD)
   apply (rule conjI, simp add: bit_simps)
   apply (clarsimp simp: pspace_distinct'_def)
@@ -216,7 +217,7 @@ lemma corres_cross_over_asid_pool_at:
 
 lemma getObject_ASIDPool_corres:
   "p' = p \<Longrightarrow>
-   corres asid_pool_relation
+   corres (\<lambda>p p'. p = inv ASIDPool p' o ucast)
           (asid_pool_at p and pspace_aligned and pspace_distinct) \<top>
           (get_asid_pool p) (getObject p')"
   apply (rule corres_cross_over_asid_pool_at, fastforce)
@@ -243,7 +244,7 @@ lemma getObject_ASIDPool_corres:
   apply (simp add: in_magnitude_check objBits_simps pageBits_def)
   apply (clarsimp simp: state_relation_def pspace_relation_def)
   apply (drule bspec, blast)
-  apply (clarsimp simp: other_aobj_relation_def)
+  apply (clarsimp simp: other_aobj_relation_def asid_pool_relation_def)
   done
 
 lemma storePTE_cte_wp_at'[wp]:
@@ -263,20 +264,13 @@ lemma storePTE_state_refs_of[wp]:
          clarsimp simp: updateObject_default_def in_monad)
   done
 
-lemma storePTE_state_hyp_refs_of[wp]:
-  "\<lbrace>\<lambda>s. P (state_hyp_refs_of' s)\<rbrace>
-     storePTE ptr val
-   \<lbrace>\<lambda>rv s. P (state_hyp_refs_of' s)\<rbrace>"
-  by (wpsimp wp: hoare_drop_imps setObject_state_hyp_refs_of_eq
-             simp: storePTE_def updateObject_default_def in_monad)
-
 crunch setIRQState
   for cte_wp_at'[wp]: "\<lambda>s. P (cte_wp_at' P' p s)"
 crunch getIRQSlot
   for inv[wp]: "P"
 
 lemma setObject_ASIDPool_corres[corres]:
-  "\<lbrakk> p = p'; a = map_option abs_asid_entry o inv ASIDPool a' o ucast \<rbrakk> \<Longrightarrow>
+  "\<lbrakk> a = inv ASIDPool a' o ucast; p' = p \<rbrakk> \<Longrightarrow>
   corres dc (asid_pool_at p and pspace_aligned and pspace_distinct) \<top>
             (set_asid_pool p a) (setObject p' a')"
   apply (simp add: set_asid_pool_def)
@@ -307,38 +301,30 @@ lemma setObject_ASIDPool_corres[corres]:
   done
 
 lemma p_le_table_base:
-  "is_aligned p pte_bits \<Longrightarrow> p + mask pte_bits \<le> table_base pt_t p + mask (table_size pt_t)"
-  apply (simp add: is_aligned_mask word_plus_and_or_coroll table_size_def pt_bits_def)
-  apply (subst word_plus_and_or_coroll, word_eqI_solve)
+  "is_aligned p pte_bits \<Longrightarrow> p + mask pte_bits \<le> table_base p + mask table_size"
+  apply (simp add: is_aligned_mask bit_simps word_plus_and_or_coroll)
   apply word_bitwise
-  apply (simp add: word_size bit_simps)
+  apply (simp add: word_size)
   done
 
-lemma table_index_in_table:
-  "table_index pt_t p \<le> mask (ptTranslationBits pt_t)"
-  by (simp add: pt_bits_def table_size_def word_bool_le_funs flip: shiftr_then_mask_commute)
-
 lemma pte_at_cross:
-  "\<lbrakk> pte_at pt_t p s; pspace_relation (kheap s) (ksPSpace s'); pspace_aligned s; pspace_distinct s \<rbrakk>
+  "\<lbrakk> pte_at p s; pspace_relation (kheap s) (ksPSpace s'); pspace_aligned s; pspace_distinct s \<rbrakk>
    \<Longrightarrow> pte_at' p s'"
   apply (drule (2) pspace_distinct_cross)
-  apply (clarsimp simp: pte_at_def ptes_of_def in_omonad obj_at_def typ_at'_def ko_wp_at'_def)
-  apply (simp split: if_split_asm)
+  apply (clarsimp simp: pte_at_def obj_at_def typ_at'_def ko_wp_at'_def)
   apply (prop_tac "p \<in> pspace_dom (kheap s)")
    apply (clarsimp simp: pspace_dom_def)
    apply (rule bexI)
     prefer 2
     apply fastforce
    apply (clarsimp simp: ran_def image_iff)
-   apply (rule_tac x="table_index pt_t p" in bexI)
-    apply (simp add: table_base_index_eq)
-   apply (simp add: table_index_in_table)
+   apply (rule_tac x="table_index p" in exI)
+   apply (simp add: mask_pt_bits_inner_beauty)
   apply (clarsimp simp: pspace_relation_def)
   apply (drule bspec, fastforce)
   apply clarsimp
-  apply (drule_tac x="table_index pt_t p" in bspec)
-   apply (simp add: table_index_in_table)
-  apply (simp add: table_base_index_eq)
+  apply (erule_tac x="table_index p" in allE)
+  apply (simp add: mask_pt_bits_inner_beauty)
   apply (clarsimp simp: pte_relation_def)
   apply (clarsimp simp: objBits_simps)
   apply (clarsimp simp: pspace_distinct'_def)
@@ -347,7 +333,7 @@ lemma pte_at_cross:
   done
 
 lemma corres_cross_over_pte_at:
-  "\<lbrakk> \<And>s. P s \<Longrightarrow> pte_at pt_t p s \<and> pspace_distinct s \<and> pspace_aligned s;
+  "\<lbrakk> \<And>s. P s \<Longrightarrow> pte_at p s \<and> pspace_distinct s \<and> pspace_aligned s;
      corres r P (P' and pte_at' p) f g\<rbrakk> \<Longrightarrow>
    corres r P P' f g"
   apply (rule corres_cross_over_guard[where Q="P' and pte_at' p"])
@@ -357,9 +343,10 @@ lemma corres_cross_over_pte_at:
   apply assumption
   done
 
-lemma getObject_PTE_corres:
-  "corres pte_relation' (pte_at pt_t p and pspace_aligned and pspace_distinct) \<top>
-          (get_pte pt_t p) (getObject p)"
+lemma getObject_PTE_corres[corres]:
+  "p = p' \<Longrightarrow>
+   corres pte_relation' (pte_at p and pspace_aligned and pspace_distinct) \<top>
+          (get_pte p) (getObject p')"
   apply (rule corres_cross_over_pte_at, fastforce)
   apply (simp add: getObject_def gets_map_def split_def bind_assoc)
   apply (rule corres_no_failI)
@@ -378,41 +365,37 @@ lemma getObject_PTE_corres:
   apply (simp add: bind_assoc exec_gets fst_assert_opt)
   apply (clarsimp simp: pte_at_eq)
   apply (clarsimp simp: ptes_of_def)
-  apply (clarsimp simp: typ_at'_def ko_wp_at'_def in_magnitude_check objBits_simps pte_bits_def word_size_bits_def)
+  apply (clarsimp simp: typ_at'_def ko_wp_at'_def in_magnitude_check objBits_simps bit_simps)
   apply (clarsimp simp: state_relation_def pspace_relation_def elim!: opt_mapE)
   apply (drule bspec, blast)
   apply (clarsimp simp: other_obj_relation_def pte_relation_def)
-  apply (drule_tac x="table_index pt_t p" in bspec)
-   apply (simp add: table_index_in_table)
-  apply (clarsimp simp: table_base_index_eq[simplified bit_simps] bit_simps)
+  apply (erule_tac x="table_index p" in allE)
+  apply (clarsimp simp: mask_pt_bits_inner_beauty[simplified bit_simps] bit_simps)
   done
 
 lemmas aligned_distinct_pte_atI'
     = aligned_distinct_obj_atI'[where 'a=pte,
                                 simplified, OF _ _ _ refl]
 
+lemma pt_bits_slot_eq:
+  "table_base p + (ucast x << pte_bits) = p \<Longrightarrow> x = ucast (p && mask table_size >> pte_bits)"
+  for x :: pt_index
+  unfolding bit_simps mask_def by word_bitwise clarsimp
+
 lemma one_less_2p_pte_bits[simp]:
   "(1::machine_word) < 2 ^ pte_bits"
   by (simp add: bit_simps)
 
-lemma pt_apply_upd_eq':
-  "idx \<le> mask (ptTranslationBits (pt_type pt)) \<Longrightarrow>
-   pt_apply (pt_upd pt (table_index (pt_type pt) p) pte) idx =
-   (if table_index (pt_type pt) p = idx then pte else pt_apply pt idx)"
-  unfolding pt_apply_def pt_upd_def
-  using table_index_mask_eq[where pt_t=NormalPT_T] table_index_mask_eq[where pt_t=VSRootPT_T]
-  by (cases pt; clarsimp simp: ucast_eq_mask vs_index_ptTranslationBits pt_index_ptTranslationBits
-                               word_le_mask_eq)
-
 \<comment> \<open>setObject_other_corres unfortunately doesn't work here\<close>
 lemma setObject_PT_corres:
   "pte_relation' pte pte' \<Longrightarrow>
-   corres dc ((\<lambda>s. pts_of s (table_base pt_t p) = Some pt) and K (is_aligned p pte_bits \<and> pt_type pt = pt_t) and
+   corres dc ((\<lambda>s. pts_of s (table_base p) = Some pt) and K (is_aligned p pte_bits) and
               pspace_aligned and pspace_distinct) \<top>
-          (set_pt (table_base pt_t p) (pt_upd pt (table_index pt_t p) pte))
+          (set_pt (table_base p) (pt(table_index p := pte)))
           (setObject p pte')"
+  supply opt_mapE[elim!]
   apply (rule corres_cross_over_pte_at[where p=p])
-   apply (fastforce simp: pte_at_eq ptes_of_def in_omonad)
+   apply (simp add: pte_at_eq ptes_of_def in_omonad)
   apply (simp add: set_pt_def get_object_def bind_assoc set_object_def gets_map_def)
   apply (rule corres_no_failI)
    apply (rule no_fail_pre, wp)
@@ -424,9 +407,8 @@ lemma setObject_PT_corres:
    apply (simp add: objBits_simps word_bits_def)
   apply (clarsimp simp: setObject_def in_monad split_def updateObject_default_def)
   apply (simp add: in_magnitude_check objBits_simps a_type_simps)
-  apply (clarsimp simp: obj_at_def exec_gets)
-  apply (clarsimp simp: exec_get put_def elim!: opt_mapE)
-  apply (clarsimp simp: state_relation_def)
+  apply (clarsimp simp: obj_at_def exec_gets a_type_simps opt_map_def exec_get put_def)
+  apply (clarsimp simp: state_relation_def mask_pt_bits_inner_beauty)
   apply (rule conjI)
    apply (clarsimp simp: pspace_relation_def split del: if_split)
    apply (rule conjI)
@@ -436,34 +418,39 @@ lemma setObject_PT_corres:
    apply (rule conjI)
     apply (drule bspec, blast)
     apply clarsimp
-    apply (drule_tac x = x in bspec)
-     apply simp
-    apply (rule conjI; clarsimp)
-     apply (clarsimp simp: pte_relation_def pt_apply_upd_eq')
-     apply (metis more_pt_inner_beauty)
-    apply (clarsimp simp: pte_relation_def table_base_index_eq pt_apply_upd_eq'
+    apply (drule_tac x = x in spec)
+    apply (clarsimp simp: pte_relation_def mask_pt_bits_inner_beauty
                    dest!: more_pt_inner_beauty)
    apply (rule ballI)
    apply (drule (1) bspec)
    apply clarsimp
    apply (rule conjI)
-    apply (clarsimp simp: pte_relation_def pt_apply_upd_eq')
-    apply (metis more_pt_inner_beauty table_base_index_eq)
+    apply (clarsimp simp: pte_relation_def mask_pt_bits_inner_beauty
+                   dest!: more_pt_inner_beauty)
    apply clarsimp
    apply (drule bspec, assumption)
    apply clarsimp
    apply (erule (1) obj_relation_cutsE)
-        apply simp
-       apply clarsimp
+       apply simp
       apply clarsimp
-      apply (smt (verit, best) pspace_aligned_pts_ofD pts_of_Some pts_of_type_unique aobjs_of_Some
-                               table_base_plus)
+     apply simp
+     apply clarsimp
+     apply (frule (1) pspace_alignedD)
+     apply (drule_tac p=x in pspace_alignedD, assumption)
+     apply simp
+     apply (drule mask_alignment_ugliness)
+        apply (simp add: pt_bits_def pageBits_def)
+       apply (simp add: pt_bits_def pageBits_def)
+      apply clarsimp
+      apply (drule test_bit_size)
+      apply (clarsimp simp: word_size bit_simps)
+      apply arith
      apply ((simp split: if_split_asm)+)[2]
     apply (simp add: other_obj_relation_def split: Structures_A.kernel_object.splits)
    apply (simp add: other_aobj_relation_def split: arch_kernel_obj.splits)
-  apply (extract_conjunct \<open>match conclusion in "ghost_relation _ _ _ _" \<Rightarrow> -\<close>)
+  apply (extract_conjunct \<open>match conclusion in "ghost_relation _ _ _" \<Rightarrow> -\<close>)
    apply (clarsimp simp add: ghost_relation_def)
-   apply (erule_tac x="p && ~~ mask (pt_bits (pt_type pt))" in allE)+
+   apply (erule_tac x="p && ~~ mask pt_bits" in allE)+
    apply fastforce
   apply (extract_conjunct \<open>match conclusion in "ready_queues_relation_2 _ _ _ _ _" \<Rightarrow> -\<close>)
    apply (prop_tac "typ_at' (koTypeOf (injectKO pte')) p b")
@@ -474,39 +461,28 @@ lemma setObject_PT_corres:
   apply (simp add: caps_of_state_after_update obj_at_def swp_cte_at_caps_of)
   done
 
-lemma storePTE_corres:
-  "pte_relation' pte pte' \<Longrightarrow>
-  corres dc (pte_at pt_t p and pspace_aligned and pspace_distinct) \<top> (store_pte pt_t p pte) (storePTE p pte')"
+lemma storePTE_corres[corres]:
+  "\<lbrakk> p = p'; pte_relation' pte pte' \<rbrakk> \<Longrightarrow>
+  corres dc (pte_at p and pspace_aligned and pspace_distinct) \<top> (store_pte p pte) (storePTE p' pte')"
   apply (simp add: store_pte_def storePTE_def)
-  apply (rule corres_assume_pre)
+  apply (rule corres_assume_pre, simp add: pte_at_def)
   apply (rule corres_symb_exec_l)
-     apply (rule corres_symb_exec_l[where P="pte_at pt_t p and pspace_aligned and pspace_distinct"])
-        apply (rule corres_symb_exec_l)
-           apply (erule setObject_PT_corres)
-          prefer 2
-          apply (rule assert_inv)
-         apply wpsimp
-        apply wpsimp
-       prefer 2
-       apply (wpsimp simp: ptes_of_def in_omonad obj_at_def pte_at_def split: if_split_asm)
-      apply (clarsimp simp: exs_valid_def gets_map_def fst_assert_opt in_omonad ptes_of_def
-                            exec_gets pte_at_def)
-     apply (wpsimp simp: pte_at_def ptes_of_def in_omonad)
-    apply (wpsimp simp: pte_at_def2)
-   apply wpsimp
-  apply (wpsimp simp: pte_at_def2)
+     apply (erule setObject_PT_corres)
+    apply (clarsimp simp: exs_valid_def gets_map_def fst_assert_opt in_omonad
+                          exec_gets bind_assoc obj_at_def pte_at_def)
+   apply (wpsimp simp: obj_at_def in_omonad)
+  apply (wpsimp simp: obj_at_def in_omonad)
   done
 
 lemmas tableBitSimps[simplified bit_simps pteBits_pte_bits, simplified] = ptBits_def
 lemmas bitSimps = tableBitSimps
 
 lemma bit_simps_corres[simp]:
-  "ptBits pt_t = pt_bits pt_t"
+  "ptBits = pt_bits"
   by (simp add: bit_simps bitSimps)
 
 defs checkPTAt_def:
-  "checkPTAt pt_t p \<equiv> stateAssert (\<lambda>s. page_table_at' pt_t p s \<and>
-                                        gsPTTypes (ksArchState s) p = Some pt_t) []"
+  "checkPTAt pt \<equiv> stateAssert (page_table_at' pt) []"
 
 lemma pte_relation_must_pte:
   "pte_relation m (ArchObj (PageTable pt)) ko \<Longrightarrow> \<exists>pte. ko = (KOArch (KOPTE pte))"
@@ -516,16 +492,16 @@ lemma pte_relation_must_pte:
   done
 
 lemma page_table_at_cross:
-  "\<lbrakk> pt_at pt_t p s; pspace_aligned s; pspace_distinct s; pspace_relation (kheap s) (ksPSpace s') \<rbrakk> \<Longrightarrow>
-   page_table_at' pt_t p s'"
+  "\<lbrakk> pt_at p s; pspace_aligned s; pspace_distinct s; pspace_relation (kheap s) (ksPSpace s') \<rbrakk> \<Longrightarrow>
+   page_table_at' p s'"
   apply (clarsimp simp: page_table_at'_def)
   apply (rule context_conjI)
    apply (clarsimp simp: obj_at_def)
    apply (frule (1) pspace_alignedD)
-   apply (clarsimp simp: bit_simps split: if_splits)
+   apply (simp add: bit_simps)
   apply clarsimp
   apply (rule pte_at_cross; assumption?)
-  apply (erule (2) page_table_pte_atI_nicer)
+  apply (clarsimp simp: obj_at_def pte_at_def table_base_plus_ucast is_aligned_pte_offset)
   done
 
 lemma getPTE_wp:
@@ -533,16 +509,32 @@ lemma getPTE_wp:
   by (clarsimp simp: getObject_def split_def loadObject_default_def in_magnitude_check
                      in_monad valid_def obj_at'_def objBits_simps)
 
-lemma check_pt_at_lift:
-  "corres_inst_eq ptr ptr' \<Longrightarrow> \<forall>s s'. (s, s') \<in> state_relation \<longrightarrow> True \<longrightarrow>
-   (pspace_aligned s \<and> pspace_distinct s \<and> pt_at pt_t ptr s \<and> ptr = ptr') \<longrightarrow>
-    \<top> s' \<longrightarrow> page_table_at' pt_t ptr' s' \<and> gsPTTypes (ksArchState s') ptr' = Some pt_t"
-  apply clarsimp
-  apply (rule conjI, fastforce intro!: page_table_at_cross)
-  by (fastforce simp: ghost_relation_def obj_at_def elim!: state_relationE)
+(* FIXME: use more recent guard crossing framework that don't need a specific goal form.
+          This was mostly left here to test compatibility bewtween corres and corresK methods *)
+(* only applies when ptr is available in abstract and concrete guard at the same time *)
+lemma pt_at_lift_eq:
+  "\<forall>s s'. (s, s') \<in> state_relation \<longrightarrow>
+          (pspace_aligned s \<and> pspace_distinct s \<and> pt_at ptr s) \<longrightarrow>
+          \<top> s' \<longrightarrow>
+          page_table_at' ptr s'"
+  by (fastforce intro!: page_table_at_cross)
 
-lemmas checkPTAt_corres[corresK] =
-  corres_stateAssert_implied_frame[OF check_pt_at_lift, folded checkPTAt_def]
+(* only applies for the "getPPtrFromHWPTE pte" pattern *)
+lemma pt_at_lift_relation:
+  "\<lbrakk> pte_relation' pte pte'; RISCV64_A.is_PageTablePTE pte \<rbrakk> \<Longrightarrow>
+   \<forall>s s'. (s, s') \<in> state_relation \<longrightarrow>
+          (pspace_aligned s \<and> pspace_distinct s \<and> pt_at (pptr_from_pte pte) s) \<longrightarrow>
+          \<top> s' \<longrightarrow>
+          page_table_at' (getPPtrFromHWPTE pte') s'"
+  apply (cases pte; simp)
+  apply (simp add: getPPtrFromHWPTE_def pptr_from_pte_def addr_from_ppn_def pt_at_lift_eq)
+  done
+
+lemmas checkPTAt_corres_pte[corres] =
+  corres_stateAssert_r_cross[OF pt_at_lift_relation, folded checkPTAt_def]
+
+lemmas checkPTAt_corres_eq[corres] =
+  corres_stateAssert_r_cross[OF pt_at_lift_eq, folded checkPTAt_def]
 
 lemma lookupPTSlotFromLevel_inv:
   "lookupPTSlotFromLevel level pt_ptr vptr \<lbrace>P\<rbrace>"
@@ -577,39 +569,34 @@ lemma ptBitsLeft_0[simp]:
 
 lemma ptBitsLeft_eq[simp]:
   "ptBitsLeft (size level) = pt_bits_left level"
-  unfolding ptBitsLeft_def pt_bits_left_def
-  by (clarsimp simp flip: vm_level.size_less_eq
-               simp: asid_pool_level_size ptTranslationBits_def maxPTLevel_def
-               split: if_splits)
+  by (simp add: ptBitsLeft_def pt_bits_left_def)
 
 lemma ptIndex_eq[simp]:
-  "ptIndex (size level) p = pt_index level p"
-  by (clarsimp simp: ptIndex_def pt_index_def levelType_def
-               simp flip: size_maxPTLevel level_type_eq(1))
+  "ptIndex (size level) = pt_index level"
+  by (fastforce simp: ptIndex_def pt_index_def)
 
 lemma ptSlotIndex_eq[simp]:
   "ptSlotIndex (size level) = pt_slot_offset level"
-  by (clarsimp intro!: ext simp: ptSlotIndex_def pt_slot_offset_def)
+  by (fastforce simp: ptSlotIndex_def pt_slot_offset_def)
 
 lemmas ptSlotIndex_0[simp] = ptSlotIndex_eq[where level=0, simplified]
 
 lemma pteAtIndex_corres:
   "level' = size level \<Longrightarrow>
    corres pte_relation'
-     (pte_at pt_t (pt_slot_offset level pt vptr) and pspace_aligned and pspace_distinct)
+     (pte_at (pt_slot_offset level pt vptr) and pspace_aligned and pspace_distinct)
      \<top>
-     (get_pte pt_t (pt_slot_offset level pt vptr))
+     (get_pte (pt_slot_offset level pt vptr))
      (pteAtIndex level' pt vptr)"
-  by (simp add: pteAtIndex_def) (rule getObject_PTE_corres)
+  by (simp add: pteAtIndex_def getObject_PTE_corres)
 
 lemma user_region_or:
   "\<lbrakk> vref \<in> user_region; vref' \<in> user_region \<rbrakk> \<Longrightarrow> vref || vref' \<in> user_region"
   by (simp add: user_region_def canonical_user_def le_mask_high_bits word_size)
 
-lemmas bit_pred = bit0.pred bit1.pred
 
-lemma lookupPTSlotFromLevel_corres:
-  "\<lbrakk> level' = size level; pt' = pt; level \<le> max_pt_level \<rbrakk> \<Longrightarrow>
+lemma lookupPTSlotFromLevel_corres[corres]:
+  "\<lbrakk> level' = size level; pt' = pt \<rbrakk> \<Longrightarrow>
    corres (\<lambda>(level, p) (bits, p'). bits = pt_bits_left level \<and> p' = p)
      (pspace_aligned and pspace_distinct and valid_vspace_objs and valid_asid_table and
      \<exists>\<rhd> (level, pt) and K (vptr \<in> user_region \<and> level \<le> max_pt_level))
@@ -624,116 +611,78 @@ next
   from `0 < level`
   obtain nlevel where nlevel: "level = nlevel + 1" by (auto intro: that[of "level-1"])
   with `0 < level`
-  have nlevel1: "nlevel < nlevel + 1" using bit_pred by fastforce
+  have nlevel1: "nlevel < nlevel + 1" using bit0.pred by fastforce
   with nlevel
   have level: "size level = Suc (size nlevel)" by simp
 
-  from `0 < level` `level \<le> max_pt_level`
-  have level_m1: "level - 1 \<le> max_pt_level"
-    by blast
-
-  from level
-  have levelType[simp]:
-    "levelType (Suc (size nlevel)) = level_type level"
-    unfolding levelType_def using vm_level.size_inj
-    by fastforce
-
   define vref_step where
-    "vref_step vref \<equiv> vref_for_level vref (level+1) || (pt_index level vptr << pt_bits_left level)"
+    "vref_step vref \<equiv>
+       vref_for_level vref (level+1) || (pt_index level vptr << pt_bits_left level)"
     for vref
 
-  from `level \<le> max_pt_level`
   have vref_for_level_step[simp]:
-    "vref_for_level (vref_step vref) (level + 1) = vref_for_level vref (level + 1)"
+    "level \<le> max_pt_level \<Longrightarrow>
+     vref_for_level (vref_step vref) (level + 1) = vref_for_level vref (level + 1)"
     for vref
     unfolding vref_step_def
-    using vref_for_level_pt_index_idem[of level level level vref vptr] by simp
+    using vref_for_level_pt_index_idem[of level level vref level vptr] by simp
 
-  from `level \<le> max_pt_level`
   have pt_walk_vref[simp]:
-    "pt_walk max_pt_level level pt (vref_step vref) =
+    "level \<le> max_pt_level \<Longrightarrow>
+     pt_walk max_pt_level level pt (vref_step vref) =
      pt_walk max_pt_level level pt vref" for pt vref
-    by - (rule pt_walk_vref_for_level_eq; simp)
+    by (rule pt_walk_vref_for_level_eq; simp)
 
-  from `level \<le> max_pt_level`
   have vref_step_user_region[simp]:
-    "\<lbrakk> vref \<in> user_region; vptr \<in> user_region \<rbrakk> \<Longrightarrow> vref_step vref \<in> user_region"
+    "\<lbrakk> vref \<in> user_region; vptr \<in> user_region; level \<le> max_pt_level \<rbrakk>
+     \<Longrightarrow> vref_step vref \<in> user_region"
     for vref
     unfolding vref_step_def
     using nlevel1 nlevel
     by (auto intro!: user_region_or vref_for_level_user_region
-             simp: pt_bits_left_def bit_simps user_region_def
+             simp: pt_bits_left_def bit_simps canonical_bit_def user_region_def
                    pt_index_def canonical_user_def word_eqI_simps
              dest!: max_pt_level_enum)
 
   have pt_slot_offset_step[simp]:
-    "\<lbrakk> is_aligned pt (pt_bits level); vref \<in> user_region \<rbrakk> \<Longrightarrow>
-     pt_slot_offset level pt (vref_step vref) = pt_slot_offset level pt vptr" for vref
+    "\<lbrakk> is_aligned pt pt_bits; vref \<in> user_region \<rbrakk> \<Longrightarrow>
+    pt_slot_offset level pt (vref_step vref) = pt_slot_offset level pt vptr" for vref
     unfolding vref_step_def using nlevel1 nlevel
-    apply simp
-    apply (clarsimp simp: pt_slot_offset_or_def user_region_def canonical_user_def)
-    apply (simp add: pt_index_def pt_bits_left_def)
-    apply (rule conjI; clarsimp)
-     apply (simp add: plus_one_eq_asid_pool vref_for_level_def pt_bits_left_def)
-     apply (rule conjI, simp add: max_pt_level_def)
-     apply (clarsimp simp: level_defs bit_simps maxPTLevel_def)
-     apply (solves \<open>cases config_ARM_PA_SIZE_BITS_40; clarsimp?; word_eqI_solve\<close>)
-    apply (clarsimp simp: vref_for_level_def pt_bits_left_def)
-    apply (rule conjI; clarsimp)
-     apply (subgoal_tac "nlevel = max_pt_level - 1")
-      apply (clarsimp simp: level_defs bit_simps maxPTLevel_def split: if_split_asm)
-      apply word_eqI_solve
-     apply (subst (asm) add.commute[where a=2])
-     apply (drule add_implies_diff)
-     apply (simp add: max_pt_level_def)
-    apply (simp add: pt_bits_def)
-    apply (prop_tac "level_type (nlevel + 1) = NormalPT_T")
-     apply (drule max_pt_level_enum)
-     (* Unfolding config_ARM_PA_SIZE_BITS_40_def here, because the level_enum only produces a
-        contradiction in one of the branches when PA_40 is set. *)
-     apply (solves \<open>auto simp: level_defs Kernel_Config.config_ARM_PA_SIZE_BITS_40_def\<close>)[1]
-    apply (simp add: bit_simps)
-    apply word_eqI
-    apply (drule max_pt_level_enum)
-    by (cases config_ARM_PA_SIZE_BITS_40, auto simp: max_pt_level_def2)
+    by (auto simp: pt_slot_offset_or_def user_region_def canonical_user_def canonical_bit_def
+                   word_eqI_simps pt_index_def bit_simps pt_bits_left_def
+             dest!: max_pt_level_enum
+             intro!: word_eqI)
 
-  from `0 < level` `level' = size level` `pt' = pt` level `level \<le> max_pt_level` level_m1
+  from `0 < level` `level' = size level` `pt' = pt` level
   show ?case
     apply (subst pt_lookup_slot_from_level_rec)
     apply (simp add: lookupPTSlotFromLevel.simps Let_def obind_comp_dist if_comp_dist
-                     gets_the_if_distrib checkPTAt_def gets_the_oapply2_comp)
+                     gets_the_if_distrib checkPTAt_def)
     apply (rule corres_guard_imp, rule corres_split[where r'=pte_relation'])
          apply (rule pteAtIndex_corres, simp)
         apply (rule corres_if3)
           apply (rename_tac pte pte', case_tac pte; (simp add: isPageTablePTE_def))
-         apply (rule corres_stateAssert_implied[where P'=\<top>])
+         apply (rule corres_stateAssert_implied)
           apply (rule minus(1))
-            apply (simp add: nlevel)
-           apply (clarsimp simp: AARCH64_A.is_PageTablePTE_def pptr_from_pte_def getPPtrFromPTE_def
-                                 paddr_from_ppn_def isPagePTE_def)
-          apply simp
+           apply (simp add: nlevel)
+          apply (clarsimp simp: RISCV64_A.is_PageTablePTE_def pptr_from_pte_def getPPtrFromHWPTE_def
+                                addr_from_ppn_def)
          apply clarsimp
-         apply (prop_tac "pt_at NormalPT_T (getPPtrFromPTE pte) s")
+         apply (rule page_table_at_cross; assumption?)
           apply (drule (2) valid_vspace_objs_strongD; assumption?)
            apply simp
-          apply (simp add: state_relation_def)
-          apply (clarsimp simp: pt_at_eq in_omonad AARCH64_A.is_PageTablePTE_def pptr_from_pte_def
-                                getPPtrFromPTE_def isPagePTE_def paddr_from_ppn_def)
-         apply (frule page_table_at_cross; assumption?)
-          apply (fastforce simp: state_relation_def)
-         apply (fastforce simp: ghost_relation_def obj_at_def elim!: state_relationE)
+          apply (clarsimp simp: pt_at_eq in_omonad RISCV64_A.is_PageTablePTE_def pptr_from_pte_def
+                                getPPtrFromHWPTE_def addr_from_ppn_def)
+         apply (simp add: state_relation_def)
         apply (rule corres_inst[where P=\<top> and P'=\<top>])
         apply (clarsimp simp: ptSlotIndex_def pt_slot_offset_def pt_index_def pt_bits_left_def
                               ptIndex_def ptBitsLeft_def)
-        apply (rule conjI; clarsimp)
-        apply (metis vm_level.size_less_eq size_maxPTLevel)
        apply wpsimp+
      apply (frule (5) vs_lookup_table_is_aligned)
      apply (rule conjI)
       apply (drule (5) valid_vspace_objs_strongD)
-      apply (clarsimp simp: pte_at_def obj_at_def ptes_of_def in_omonad)
+      apply (clarsimp simp: pte_at_def obj_at_def elim!: opt_mapE)
       apply (simp add: pt_slot_offset_def)
-      apply (rule conjI, fastforce)
       apply (rule is_aligned_add)
        apply (erule is_aligned_weaken)
        apply (simp add: bit_simps)
@@ -745,7 +694,7 @@ next
      apply (rule conjI)
       apply (clarsimp simp: level_defs)
      apply (subst pt_walk_split_Some[where level'=level]; simp?)
-      apply (drule vm_level.pred)
+      apply (drule bit0.pred)
       apply simp
      apply (subst pt_walk.simps)
      apply (simp add: in_omonad)
@@ -761,15 +710,13 @@ lemma lookupPTSlot_corres:
           \<top>
           (gets_the (pt_lookup_slot pt vptr \<circ> ptes_of)) (lookupPTSlot pt vptr)"
   unfolding lookupPTSlot_def pt_lookup_slot_def
-  apply (corresKsimp corres: lookupPTSlotFromLevel_corres)
-  apply (fastforce simp: vspace_pt_at_eq pt_type_def
-                   dest!: valid_vspace_objs_strongD
-                   split: pt.splits)
-  done
+  by corres
+
+declare RISCV64_A.pte.sel[datatype_schematic]
 
 lemma lookupPTFromLevel_corres:
   "\<lbrakk> level' = size level; pt' = pt \<rbrakk> \<Longrightarrow>
-   corres (lfr \<oplus> ((=) \<circ> fst))
+   corres (lfr \<oplus> (=))
           (pspace_aligned and pspace_distinct and valid_vspace_objs
              and valid_asid_table and \<exists>\<rhd>(level,pt)
              and K (vptr \<in> user_region \<and> level \<le> max_pt_level \<and> pt \<noteq> target))
@@ -787,11 +734,13 @@ proof (induct level arbitrary: level' pt pt')
 next
   case (minus level)
 
+  note minus.hyps(1)[corres]
+
   (* FIXME: unfortunate duplication from lookupPTSlotFromLevel_corres *)
   from `0 < level`
   obtain nlevel where nlevel: "level = nlevel + 1" by (auto intro: that[of "level-1"])
   with `0 < level`
-  have nlevel1: "nlevel < nlevel + 1" using vm_level.pred by fastforce
+  have nlevel1: "nlevel < nlevel + 1" using bit0.pred by fastforce
   with nlevel
   have level: "size level = Suc (size nlevel)" by simp
 
@@ -805,7 +754,7 @@ next
      vref_for_level (vref_step vref) (level + 1) = vref_for_level vref (level + 1)"
     for vref
     unfolding vref_step_def
-    using vref_for_level_pt_index_idem[of level level level vref vptr] by simp
+    using vref_for_level_pt_index_idem[of level level vref level vptr] by simp
 
   have pt_walk_vref[simp]:
     "level \<le> max_pt_level \<Longrightarrow>
@@ -820,101 +769,56 @@ next
     unfolding vref_step_def
     using nlevel1 nlevel
     by (auto intro!: user_region_or vref_for_level_user_region
-             simp: pt_bits_left_def bit_simps user_region_def
+             simp: pt_bits_left_def bit_simps canonical_bit_def user_region_def
                    pt_index_def canonical_user_def word_eqI_simps
              dest!: max_pt_level_enum)
 
   have pt_slot_offset_step[simp]:
-    "\<lbrakk> is_aligned pt (pt_bits level); vref \<in> user_region \<rbrakk> \<Longrightarrow>
+    "\<lbrakk> is_aligned pt pt_bits; vref \<in> user_region \<rbrakk> \<Longrightarrow>
     pt_slot_offset level pt (vref_step vref) = pt_slot_offset level pt vptr" for vref
     unfolding vref_step_def using nlevel1 nlevel
-    apply simp
-    apply (clarsimp simp: pt_slot_offset_or_def user_region_def canonical_user_def)
-    apply (simp add: pt_index_def pt_bits_left_def)
-    apply (rule conjI; clarsimp)
-     apply (simp add: plus_one_eq_asid_pool vref_for_level_def pt_bits_left_def)
-     apply (rule conjI, simp add: max_pt_level_def)
-     apply (clarsimp simp: level_defs bit_simps maxPTLevel_def)
-     apply (solves \<open>cases config_ARM_PA_SIZE_BITS_40; clarsimp?; word_eqI_solve\<close>)
-    apply (clarsimp simp: vref_for_level_def pt_bits_left_def)
-    apply (rule conjI; clarsimp)
-     apply (subgoal_tac "nlevel = max_pt_level - 1")
-      apply (clarsimp simp: level_defs bit_simps maxPTLevel_def split: if_split_asm)
-      apply word_eqI_solve
-     apply (subst (asm) add.commute[where a=2])
-     apply (drule add_implies_diff)
-     apply (simp add: max_pt_level_def)
-    apply (simp add: pt_bits_def)
-    apply (prop_tac "level_type (nlevel + 1) = NormalPT_T")
-     apply (drule max_pt_level_enum)
-     (* Unfolding config_ARM_PA_SIZE_BITS_40_def here, because the level_enum only produces a
-        contradiction in one of the branches when PA_40 is set. *)
-     apply (solves \<open>auto simp: level_defs Kernel_Config.config_ARM_PA_SIZE_BITS_40_def split: if_split_asm\<close>)[1]
-    apply (simp add: bit_simps)
-    apply word_eqI
-    apply (drule max_pt_level_enum)
-    by (cases config_ARM_PA_SIZE_BITS_40, auto simp: max_pt_level_def2)
+    by (auto simp: pt_slot_offset_or_def user_region_def canonical_user_def canonical_bit_def
+                   word_eqI_simps pt_index_def bit_simps pt_bits_left_def
+             dest!: max_pt_level_enum
+             intro!: word_eqI)
 
-  note vm_level.size_minus_one[simp]
+  note bit0.size_minus_one[simp]
   from minus.prems
   show ?case
     apply (subst lookupPTFromLevel.simps, subst pt_lookup_from_level_simps)
     apply (simp add: unlessE_whenE not_less)
     apply (rule corres_gen_asm, simp)
-    apply (rule corres_initial_splitE[where r'=dc])
-       apply (corresKsimp simp: lookup_failure_map_def)
-      apply (rule corres_splitEE[where r'=pte_relation'])
-         apply (simp, rule getObject_PTE_corres)
-        apply (rule whenE_throwError_corres)
-          apply (simp add: lookup_failure_map_def)
+    apply (corres simp: lookup_failure_map_def)
          apply (rename_tac pte pte', case_tac pte; simp add: isPageTablePTE_def)
-        apply (rule corres_if)
-          apply (clarsimp simp: AARCH64_A.is_PageTablePTE_def pptr_from_pte_def getPPtrFromPTE_def
-                                paddr_from_ppn_def isPagePTE_def)
-         apply (rule corres_returnOk[where P=\<top> and P'=\<top>], simp)
-        apply (clarsimp simp: checkPTAt_def)
-        apply (subst liftE_bindE, rule corres_stateAssert_implied[where P'=\<top>])
-         apply (rule minus.hyps)
-          apply (simp add: minus.hyps(2))
-         apply (clarsimp simp: AARCH64_A.is_PageTablePTE_def pptr_from_pte_def getPPtrFromPTE_def
-                               paddr_from_ppn_def isPagePTE_def)
-        apply clarsimp
-        apply (prop_tac "pt_at NormalPT_T (pptr_from_pte pte) s")
-         apply (drule (2) valid_vspace_objs_strongD; assumption?)
-          apply simp
-         apply (simp add: state_relation_def)
-         apply (clarsimp simp: pt_at_eq in_omonad AARCH64_A.is_PageTablePTE_def pptr_from_pte_def
-                               getPPtrFromPTE_def isPagePTE_def paddr_from_ppn_def)
-        apply (frule page_table_at_cross; assumption?)
-         apply (fastforce simp: state_relation_def)
-        apply (clarsimp simp: AARCH64_A.is_PageTablePTE_def pptr_from_pte_def getPPtrFromPTE_def
-                              paddr_from_ppn_def isPagePTE_def)
-        apply (fastforce simp: ghost_relation_def obj_at_def
-                         elim!: state_relationE)
+        apply (corres term_simp: RISCV64_A.is_PageTablePTE_def pptr_from_pte_def
+                                 getPPtrFromHWPTE_def addr_from_ppn_def minus.hyps(2))
        apply wpsimp+
-     apply (simp add: vm_level.neq_0_conv)
+     apply (simp add: bit0.neq_0_conv)
      apply (frule (5) vs_lookup_table_is_aligned)
      apply (rule conjI)
       apply (drule (5) valid_vspace_objs_strongD)
-      apply (clarsimp simp: pte_at_def obj_at_def ptes_of_def in_omonad)
-      apply (rule conjI, fastforce)
+      apply (clarsimp simp: pte_at_def obj_at_def elim!: opt_mapE)
       apply (simp add: pt_slot_offset_def)
       apply (rule is_aligned_add)
        apply (erule is_aligned_weaken)
        apply (simp add: bit_simps)
       apply (rule is_aligned_shiftl, simp)
      apply clarsimp
-     apply (rule_tac x=asid in exI)
-     apply (rule_tac x="vref_step vref" in exI)
-     apply (clarsimp simp: vs_lookup_table_def in_omonad split: if_split_asm)
      apply (rule conjI)
-      apply (clarsimp simp: level_defs)
-     apply (subst pt_walk_split_Some[where level'=level]; simp?)
-      apply (drule vm_level.pred)
-      apply simp
-     apply (subst pt_walk.simps)
-     apply (simp add: in_omonad)
-    apply wpsimp
+      apply (rule_tac x=asid in exI)
+      apply (rule_tac x="vref_step vref" in exI)
+      apply (clarsimp simp: vs_lookup_table_def in_omonad split: if_split_asm)
+      apply (rule conjI)
+       apply (clarsimp simp: level_defs)
+      apply (subst pt_walk_split_Some[where level'=level]; simp?)
+       apply (drule bit0.pred)
+       apply simp
+      apply (subst pt_walk.simps)
+      apply (simp add: in_omonad)
+     apply (drule (1) valid_vspace_objs_pte, fastforce)
+     apply (clarsimp simp: RISCV64_A.is_PageTablePTE_def pptr_from_pte_def
+                           table_index_max_level_slots)
+    apply simp
     done
 qed
 
@@ -936,19 +840,40 @@ lemma getObject_pte_inv[wp]:
   "\<lbrace>P\<rbrace> getObject p \<lbrace>\<lambda>rv :: pte. P\<rbrace>"
   by (simp add: getObject_inv loadObject_default_inv)
 
+crunch copyGlobalMappings
+  for typ_at'[wp]: "\<lambda>s. P (typ_at' T p s)"
+  (wp: mapM_x_wp')
+
+lemmas copyGlobalMappings_typ_ats[wp] = typ_at_lifts [OF copyGlobalMappings_typ_at']
+
 lemma corres_gets_global_pt [corres]:
   "corres (=) valid_global_arch_objs \<top>
-              (gets global_pt) (gets (armKSGlobalUserVSpace \<circ> ksArchState))"
-  by (clarsimp simp add: state_relation_def arch_state_relation_def)
+              (gets global_pt) (gets (riscvKSGlobalPT \<circ> ksArchState))"
+  apply (clarsimp simp add: state_relation_def arch_state_relation_def riscv_global_pt_def
+                            riscvKSGlobalPT_def valid_global_arch_objs_def)
+  apply (case_tac "riscvKSGlobalPTs (ksArchState s') maxPTLevel"; simp)
+  done
 
-lemmas getObject_PTE_corres'[corres] = getObject_PTE_corres[@lift_corres_args]
-lemmas storePTE_corres'[corres] = storePTE_corres[@lift_corres_args]
+lemma copy_global_mappings_corres [@lift_corres_args, corres]:
+  "corres dc (valid_global_arch_objs and pspace_aligned and pspace_distinct and pt_at pt)
+             \<top>
+             (copy_global_mappings pt)
+             (copyGlobalMappings pt)" (is "corres _ ?apre _ _ _")
+  unfolding copy_global_mappings_def copyGlobalMappings_def objBits_simps archObjSize_def pptr_base_def
+  apply corres
+      apply (rule_tac P="pt_at global_pt and ?apre" and P'="\<top>" in corres_mapM_x[OF _ _ _ _ order_refl])
+         apply (corres simp: ptIndex_def ptBitsLeft_def maxPTLevel_def ptTranslationBits_def pageBits_def
+                             pt_index_def pt_bits_left_def level_defs
+                | fastforce dest!: valid_global_arch_objs_pt_at
+                            intro!: page_table_pte_atI
+                            simp: bit_simps word_le_nat_alt word_less_nat_alt)+
+  done
 
 lemma arch_cap_rights_update:
   "acap_relation c c' \<Longrightarrow>
    cap_relation (cap.ArchObjectCap (acap_rights_update (acap_rights c \<inter> msk) c))
                  (Arch.maskCapRights (rights_mask_map msk) c')"
-  apply (cases c, simp_all add: AARCH64_H.maskCapRights_def
+  apply (cases c, simp_all add: RISCV64_H.maskCapRights_def
                                 acap_rights_update_def Let_def isCap_simps)
   apply (simp add: maskVMRights_def vmrights_map_def rights_mask_map_def
                    validate_vm_rights_def vm_read_write_def vm_read_only_def
@@ -957,7 +882,7 @@ lemma arch_cap_rights_update:
 
 lemma arch_deriveCap_inv:
   "\<lbrace>P\<rbrace> Arch.deriveCap arch_cap u \<lbrace>\<lambda>rv. P\<rbrace>"
-  apply (simp      add: AARCH64_H.deriveCap_def
+  apply (simp      add: RISCV64_H.deriveCap_def
                   cong: if_cong
              split del: if_split)
   apply (wp undefined_valid)
@@ -968,10 +893,10 @@ lemma arch_deriveCap_valid:
   "\<lbrace>valid_cap' (ArchObjectCap arch_cap)\<rbrace>
      Arch.deriveCap u arch_cap
    \<lbrace>\<lambda>rv. valid_cap' rv\<rbrace>,-"
-  apply (simp add: AARCH64_H.deriveCap_def split del: if_split)
+  apply (simp add: RISCV64_H.deriveCap_def split del: if_split)
   apply (wp undefined_validE_R)
   apply (cases arch_cap; simp add: isCap_defs)
-  apply (simp add: valid_cap'_def capAligned_def capUntypedPtr_def AARCH64_H.capUntypedPtr_def)
+  apply (simp add: valid_cap'_def capAligned_def capUntypedPtr_def RISCV64_H.capUntypedPtr_def)
   done
 
 lemma mdata_map_simps[simp]:
@@ -985,16 +910,17 @@ lemma arch_deriveCap_corres:
          \<top> \<top>
          (arch_derive_cap c)
          (Arch.deriveCap slot c')"
-  unfolding arch_derive_cap_def AARCH64_H.deriveCap_def Let_def
+  unfolding arch_derive_cap_def RISCV64_H.deriveCap_def Let_def
   apply (cases c, simp_all add: isCap_simps split: option.splits split del: if_split)
       apply (clarify?, rule corres_noopE; wpsimp)+
   done
 
+
 definition
-  "vmattributes_map \<equiv> \<lambda>R. VMAttributes (Execute \<notin> R) (Device \<notin> R)"
+  "vmattributes_map \<equiv> \<lambda>R. VMAttributes (Execute \<notin> R)"
 
 lemma pte_relation'_Invalid_inv [simp]:
-  "pte_relation' x AARCH64_H.pte.InvalidPTE = (x = AARCH64_A.pte.InvalidPTE)"
+  "pte_relation' x RISCV64_H.pte.InvalidPTE = (x = RISCV64_A.pte.InvalidPTE)"
   by (cases x) auto
 
 lemma asidHighBitsOf [simp]:
@@ -1013,83 +939,43 @@ lemma asid_case_zero[simp]:
   "0 < asid \<Longrightarrow> 0 < UCAST(asid_len \<rightarrow> machine_word_len) asid"
   by word_bitwise
 
+lemma gets_opt_bind_throw_opt:
+  "(gets (do { x \<leftarrow> f; g x }) >>= throw_opt E) =
+   (do x_opt \<leftarrow> gets f;
+       doE x \<leftarrow> throw_opt E x_opt;
+           gets (g x) >>= throw_opt E
+       odE
+    od)"
+  apply (rule ext)
+  apply (simp add: bind_def simpler_gets_def throw_opt_def)
+  apply (simp add: obind_def split: option.splits)
+  done
+
 lemma find_vspace_for_asid_rewite:
-  "find_vspace_for_asid asid =
-   doE
-     unlessE (0 < asid) $ throwError ExceptionTypes_A.InvalidRoot;
-     entry_opt \<leftarrow> liftE $ gets (entry_for_asid asid);
-     case entry_opt of
-       Some entry \<Rightarrow> returnOk (ap_vspace entry)
-     | None \<Rightarrow> throwError ExceptionTypes_A.InvalidRoot
-   odE"
-  unfolding find_vspace_for_asid_def vspace_for_asid_def
-  apply (cases "0 < asid")
-   apply simp (* rewrite unlessE before unfolding things *)
-   apply (fastforce simp: bindE_def throw_opt_def liftE_def simpler_gets_def bind_def return_def
-                          obind_None_eq
-                    split: option.splits)
-  apply (simp add: liftE_def simpler_gets_def bindE_def bind_def return_def throw_opt_def
-                   throwError_def)
+  "monadic_rewrite False True (valid_asid_table and K (0 < asid))
+     (find_vspace_for_asid asid)
+     (doE
+        asid_table \<leftarrow> liftE $ gets (riscv_asid_table \<circ> arch_state);
+        pool_ptr \<leftarrow> returnOk (asid_table (asid_high_bits_of asid));
+        pool \<leftarrow> (case pool_ptr of
+                  Some ptr \<Rightarrow> liftE $ get_asid_pool ptr
+                | None \<Rightarrow> throwError ExceptionTypes_A.InvalidRoot);
+        pt \<leftarrow> returnOk (pool (ucast asid));
+        (case pt of
+            Some ptr \<Rightarrow> returnOk ptr
+          | None \<Rightarrow> throwError ExceptionTypes_A.InvalidRoot)
+      odE)"
+  unfolding find_vspace_for_asid_def vspace_for_asid_def pool_for_asid_def vspace_for_pool_def
+  apply (clarsimp simp: monadic_rewrite_def)
+  apply (simp add: gets_opt_bind_throw_opt liftE_bindE obind_comp_dist gets_map_def cong: option.case_cong)
+  apply (clarsimp simp: o_def exec_gets throw_opt_def split: option.splits)
+  apply (rule conjI; clarsimp)
+   apply (drule (1) valid_asid_tableD)
+   apply (clarsimp simp: obj_at_def opt_map_def)
+  apply (simp add: liftE_bindE bind_assoc exec_gets opt_map_def asid_low_bits_of_def)
   done
 
-lemma getPoolPtr_corres:
-  "corres (=) (K (0 < asid)) \<top> (gets (pool_for_asid asid)) (getPoolPtr (ucast asid))"
-  unfolding pool_for_asid_def getPoolPtr_def asidRange_def
-  apply simp
-  apply corres_pre
-    apply (rule corres_assert_gen_asm)
-    apply (rule corres_assert_gen_asm)
-    apply (rule corres_trivial)
-    apply (clarsimp simp: gets_return_gets_eq state_relation_def arch_state_relation_def
-                          ucast_up_ucast_id is_up)
-   apply (simp flip: mask_eq_exp_minus_1)
-  apply simp
-  done
-
-lemma getASIDPoolEntry_corres:
-  "corres (\<lambda>r r'. r = map_option abs_asid_entry r')
-          (valid_vspace_objs and valid_asid_table and pspace_aligned and pspace_distinct
-           and K (0 < asid))
-          (no_0_obj')
-          (gets (entry_for_asid asid))
-          (getASIDPoolEntry (ucast asid))"
-  unfolding entry_for_asid_def getASIDPoolEntry_def K_def
-  apply (rule corres_gen_asm)
-  apply (clarsimp simp: gets_obind_bind_eq entry_for_pool_def obind_comp_dist
-                  cong: option.case_cong)
-  apply (rule corres_guard_imp)
-    apply (rule corres_split[where r'="(=)"])
-       apply (rule getPoolPtr_corres)
-      apply (rule_tac x=pool_ptr and x'=poolPtr in option_corres)
-        apply (rule corres_trivial, simp)
-       apply clarsimp
-       apply (rule monadic_rewrite_corres_l)
-        apply (monadic_rewrite_l gets_oapply_liftM_rewrite)
-        apply (rule monadic_rewrite_refl)
-       apply (clarsimp simp: liftM_def)
-       apply (rule corres_split[OF getObject_ASIDPool_corres[OF refl]])
-         apply (rule corres_trivial)
-         apply (case_tac rv', clarsimp)
-         apply (clarsimp simp: asid_pool_relation_def asid_low_bits_of_def ucast_ucast_mask2
-                               is_down asid_low_bits_def ucast_and_mask)
-        apply wpsimp+
-   apply (drule (1) pool_for_asid_validD)
-   apply (simp add: asid_pools_at_eq)
-  apply simp
-  done
-
-lemma no_0_page_table:
-  "\<lbrakk> no_0_obj' s; page_table_at' pt_t 0 s \<rbrakk> \<Longrightarrow> False"
-  apply (clarsimp simp: page_table_at'_def)
-  apply (erule_tac x=0 in allE)
-  apply simp
-  done
-
-crunch getASIDPoolEntry
-  for no_0_obj'[wp]: no_0_obj'
-  (wp: getObject_inv simp: loadObject_default_def)
-
-lemma findVSpaceForASID_corres:
+lemma findVSpaceForASID_corres[corres]:
   assumes "asid' = ucast asid"
   shows "corres (lfr \<oplus> (=))
                 (valid_vspace_objs and valid_asid_table
@@ -1099,40 +985,47 @@ lemma findVSpaceForASID_corres:
                 (find_vspace_for_asid asid) (findVSpaceForASID asid')" (is "corres _ ?P ?Q _ _")
   using assms
   apply (simp add: findVSpaceForASID_def)
-  apply (rule corres_gen_asm)
-  apply (subst find_vspace_for_asid_rewite)
-  apply clarsimp
+  apply (rule corres_gen_asm, simp add: ucast_down_ucast_id is_down_def target_size source_size)
+  apply (rule corres_guard_imp[where Q'="?Q"], rule monadic_rewrite_corres_l[where P="?P"],
+         rule find_vspace_for_asid_rewite; simp)
+  apply (simp add: liftE_bindE asidRange_def flip: mask_2pm1)
+  apply (rule_tac r'="\<lambda>x y. x = y o ucast"
+             in corres_underlying_split [OF _ _ gets_sp gets_sp])
+   apply (clarsimp simp: state_relation_def arch_state_relation_def)
+  apply (case_tac "rv (asid_high_bits_of asid)")
+   apply (simp add: liftME_def lookup_failure_map_def)
+  apply (simp add: liftME_def bindE_assoc)
+  apply (simp add: liftE_bindE)
   apply (rule corres_guard_imp)
-    apply (rule corres_initial_splitE[where r'="\<lambda>r r'. r = map_option abs_asid_entry r'"])
-       apply simp
-       apply (rule getASIDPoolEntry_corres)
-      apply (rule_tac Q="\<lambda>entry s. pspace_aligned s \<and> pspace_distinct s \<and>
-                                   vspace_pt_at (ap_vspace entry) s"
-                      in option_corres[where P=\<top> and P'=\<top> and Q'="\<lambda>_. no_0_obj'"])
-        apply (clarsimp simp: lookup_failure_map_def)
-       apply (rename_tac entry entry')
-       apply (case_tac entry')
-       apply (clarsimp simp: checkPTAt_def abs_asid_entry_def)
-       apply (rename_tac p)
-       apply (rule_tac Q="\<lambda>s. page_table_at' VSRootPT_T p s \<and>
-                              gsPTTypes (ksArchState s) p = Some VSRootPT_T \<and>
-                              no_0_obj' s" in corres_cross_over_guard)
-        apply clarsimp
-        apply (rule conjI)
-         apply (erule (2) page_table_at_cross, simp add: state_relation_def)
-        apply (fastforce simp: ghost_relation_def obj_at_def elim!: state_relationE)
-       apply (simp add: liftE_bindE assertE_liftE)
-       apply (rule corres_assert_assume)
-        apply (rule corres_stateAssert_assume)
-         apply (rule corres_returnOk, simp)
-        apply clarsimp
-       apply (fastforce dest: no_0_page_table)
-      apply simp
-     apply wpsimp
-     apply (clarsimp simp: entry_for_asid_def)
-     apply (drule (2) pool_for_asid_valid_vspace_objs)
-     apply (fastforce simp: entry_for_pool_def)
-    apply (wpsimp wp: hoare_drop_imps)+
+    apply (rule corres_split[OF getObject_ASIDPool_corres[OF refl]])
+      apply (rule_tac P="case_option \<top> pt_at (pool (ucast asid)) and pspace_aligned and pspace_distinct"
+                 and P'="no_0_obj'" in corres_inst)
+      apply (rule_tac F="pool (ucast asid) \<noteq> Some 0" in corres_req)
+       apply (clarsimp simp: obj_at_def no_0_obj'_def state_relation_def
+                             pspace_relation_def a_type_def)
+       apply (simp split: Structures_A.kernel_object.splits
+                          arch_kernel_obj.splits if_split_asm)
+       apply (drule_tac f="\<lambda>S. 0 \<in> S" in arg_cong)
+       apply (simp add: pspace_dom_def)
+       apply (drule iffD1, rule rev_bexI, erule domI)
+        apply simp
+        apply (rule image_eqI[rotated])
+         apply (rule rangeI[where x=0])
+        apply simp
+       apply clarsimp
+      apply (simp add: mask_asid_low_bits_ucast_ucast asid_low_bits_of_def returnOk_def
+                       lookup_failure_map_def ucast_ucast_a is_down
+                  split: option.split)
+      apply (corres corres: corres_returnTT)
+     apply (wpsimp wp: getObject_inv loadObject_default_inv)+
+   apply (clarsimp simp: o_def)
+   apply (rule conjI)
+    apply (rule valid_asid_tableD; simp)
+   apply (clarsimp split: option.splits)
+   apply (rule vs_lookup_table_pt_at[where vptr=0 and level=max_pt_level and asid=asid]; simp?)
+   apply (simp add: vs_lookup_table_def pool_for_asid_def vspace_for_pool_def in_omonad obj_at_def
+                    asid_low_bits_of_def)
+  apply simp
   done
 
 lemma setObject_arch:
@@ -1159,14 +1052,12 @@ lemma setObject_PTE_arch [wp]:
   done
 
 lemma setObject_ASID_valid_arch [wp]:
-  "setObject p (v::asidpool) \<lbrace>valid_arch_state'\<rbrace>"
-  by (wpsimp wp: valid_arch_state_lift' setObject_ko_wp_at)
-     (auto simp: objBits_simps pageBits_def is_vcpu'_def ko_wp_at'_def obj_at'_def)
+  "\<lbrace>valid_arch_state'\<rbrace> setObject p (v::asidpool) \<lbrace>\<lambda>_. valid_arch_state'\<rbrace>"
+  by (rule valid_arch_state_lift'; wp)
 
 lemma setObject_PTE_valid_arch [wp]:
   "\<lbrace>valid_arch_state'\<rbrace> setObject p (v::pte) \<lbrace>\<lambda>_. valid_arch_state'\<rbrace>"
-  by (wpsimp wp: valid_arch_state_lift' setObject_typ_at' setObject_ko_wp_at)
-     (auto simp: objBits_simps pageBits_def is_vcpu'_def ko_wp_at'_def obj_at'_def)
+  by (rule valid_arch_state_lift') (wp setObject_typ_at')+
 
 lemma setObject_ASID_ct [wp]:
   "\<lbrace>\<lambda>s. P (ksCurThread s)\<rbrace> setObject p (e::asidpool) \<lbrace>\<lambda>_ s. P (ksCurThread s)\<rbrace>"
